secret integers in fstar

hax-secret-integers/src/lib.rs
@@ -1,12 +1,12 @@
 mod traits;
 pub use traits::*;
 
-#[cfg(feature = "secret_independence")]
+#[cfg(all(hax,feature = "secret_independence"))]
 mod secret_integers;
-#[cfg(feature = "secret_independence")]
+#[cfg(all(hax,feature = "secret_independence"))]
 pub use secret_integers::*;
 
-#[cfg(not(feature = "secret_independence"))]
+#[cfg(not(all(hax,feature = "secret_independence")))]
 mod public_integers;
-#[cfg(not(feature = "secret_independence"))]
+#[cfg(not(all(hax,feature = "secret_independence")))]
 pub use public_integers::*;
