examples/chacha20/proofs/fstar/extraction/Chacha20.fst
@@ -3,112 +3,59 @@ module Chacha20
 open Core
 open FStar.Mul
 
-unfold
-let t_Block = t_Array u8 (sz 64)
+let _ =
+  (* This module has implicit dependencies, here we make them explicit. *)
+  (* The implicit dependencies arise from typeclasses instances. *)
+  let open Hax_secret_integers.Public_integers in
+  ()
 
-unfold
-let t_ChaChaIV = t_Array u8 (sz 12)
-
-unfold
-let t_ChaChaKey = t_Array u8 (sz 32)
-
-unfold
-let t_State = t_Array u32 (sz 16)
-
-unfold
-let t_StateIdx = Hax_bounded_integers.t_BoundedUsize (sz 0) (sz 15)
-
-let chacha20_line
-      (a b d: Hax_bounded_integers.t_BoundedUsize (sz 0) (sz 15))
-      (s: u32)
-      (m: t_Array u32 (sz 16))
-    : t_Array u32 (sz 16) =
+let chacha20_line (a b d: usize) (s: u32) (m: t_Array u32 (sz 16))
+    : Prims.Pure (t_Array u32 (sz 16))
+      (requires a <. sz 16 && b <. sz 16 && d <. sz 16)
+      (fun _ -> Prims.l_True) =
   let state:t_Array u32 (sz 16) = m in
   let state:t_Array u32 (sz 16) =
-    Rust_primitives.Hax.update_at state
+    Rust_primitives.Hax.Monomorphized_update_at.update_at_usize state
       a
       (Core.Num.impl__u32__wrapping_add (state.[ a ] <: u32) (state.[ b ] <: u32) <: u32)
   in
   let state:t_Array u32 (sz 16) =
-    Rust_primitives.Hax.update_at state d ((state.[ d ] <: u32) ^. (state.[ a ] <: u32) <: u32)
+    Rust_primitives.Hax.Monomorphized_update_at.update_at_usize state
+      d
+      ((state.[ d ] <: u32) ^. (state.[ a ] <: u32) <: u32)
   in
   let state:t_Array u32 (sz 16) =
-    Rust_primitives.Hax.update_at state
+    Rust_primitives.Hax.Monomorphized_update_at.update_at_usize state
       d
       (Core.Num.impl__u32__rotate_left (state.[ d ] <: u32) s <: u32)
   in
   state
 
-let chacha20_quarter_round
-      (a b c d: Hax_bounded_integers.t_BoundedUsize (sz 0) (sz 15))
-      (state: t_Array u32 (sz 16))
-    : t_Array u32 (sz 16) =
+let chacha20_quarter_round (a b c d: usize) (state: t_Array u32 (sz 16))
+    : Prims.Pure (t_Array u32 (sz 16))
+      (requires a <. sz 16 && b <. sz 16 && c <. sz 16 && d <. sz 16)
+      (fun _ -> Prims.l_True) =
   let state:t_Array u32 (sz 16) = chacha20_line a b d 16ul state in
   let state:t_Array u32 (sz 16) = chacha20_line c d b 12ul state in
   let state:t_Array u32 (sz 16) = chacha20_line a b d 8ul state in
   chacha20_line c d b 7ul state
 
 let chacha20_double_round (state: t_Array u32 (sz 16)) : t_Array u32 (sz 16) =
-  let state:t_Array u32 (sz 16) =
-    chacha20_quarter_round (sz 0 <: Hax_bounded_integers.t_BoundedUsize (sz 0) (sz 15))
-      (sz 4 <: Hax_bounded_integers.t_BoundedUsize (sz 0) (sz 15))
-      (sz 8 <: Hax_bounded_integers.t_BoundedUsize (sz 0) (sz 15))
-      (sz 12 <: Hax_bounded_integers.t_BoundedUsize (sz 0) (sz 15))
-      state
-  in
-  let state:t_Array u32 (sz 16) =
-    chacha20_quarter_round (sz 1 <: Hax_bounded_integers.t_BoundedUsize (sz 0) (sz 15))
-      (sz 5 <: Hax_bounded_integers.t_BoundedUsize (sz 0) (sz 15))
-      (sz 9 <: Hax_bounded_integers.t_BoundedUsize (sz 0) (sz 15))
-      (sz 13 <: Hax_bounded_integers.t_BoundedUsize (sz 0) (sz 15))
-      state
-  in
-  let state:t_Array u32 (sz 16) =
-    chacha20_quarter_round (sz 2 <: Hax_bounded_integers.t_BoundedUsize (sz 0) (sz 15))
-      (sz 6 <: Hax_bounded_integers.t_BoundedUsize (sz 0) (sz 15))
-      (sz 10 <: Hax_bounded_integers.t_BoundedUsize (sz 0) (sz 15))
-      (sz 14 <: Hax_bounded_integers.t_BoundedUsize (sz 0) (sz 15))
-      state
-  in
-  let state:t_Array u32 (sz 16) =
-    chacha20_quarter_round (sz 3 <: Hax_bounded_integers.t_BoundedUsize (sz 0) (sz 15))
-      (sz 7 <: Hax_bounded_integers.t_BoundedUsize (sz 0) (sz 15))
-      (sz 11 <: Hax_bounded_integers.t_BoundedUsize (sz 0) (sz 15))
-      (sz 15 <: Hax_bounded_integers.t_BoundedUsize (sz 0) (sz 15))
-      state
-  in
-  let state:t_Array u32 (sz 16) =
-    chacha20_quarter_round (sz 0 <: Hax_bounded_integers.t_BoundedUsize (sz 0) (sz 15))
-      (sz 5 <: Hax_bounded_integers.t_BoundedUsize (sz 0) (sz 15))
-      (sz 10 <: Hax_bounded_integers.t_BoundedUsize (sz 0) (sz 15))
-      (sz 15 <: Hax_bounded_integers.t_BoundedUsize (sz 0) (sz 15))
-      state
-  in
-  let state:t_Array u32 (sz 16) =
-    chacha20_quarter_round (sz 1 <: Hax_bounded_integers.t_BoundedUsize (sz 0) (sz 15))
-      (sz 6 <: Hax_bounded_integers.t_BoundedUsize (sz 0) (sz 15))
-      (sz 11 <: Hax_bounded_integers.t_BoundedUsize (sz 0) (sz 15))
-      (sz 12 <: Hax_bounded_integers.t_BoundedUsize (sz 0) (sz 15))
-      state
-  in
-  let state:t_Array u32 (sz 16) =
-    chacha20_quarter_round (sz 2 <: Hax_bounded_integers.t_BoundedUsize (sz 0) (sz 15))
-      (sz 7 <: Hax_bounded_integers.t_BoundedUsize (sz 0) (sz 15))
-      (sz 8 <: Hax_bounded_integers.t_BoundedUsize (sz 0) (sz 15))
-      (sz 13 <: Hax_bounded_integers.t_BoundedUsize (sz 0) (sz 15))
-      state
-  in
-  chacha20_quarter_round (sz 3 <: Hax_bounded_integers.t_BoundedUsize (sz 0) (sz 15))
-    (sz 4 <: Hax_bounded_integers.t_BoundedUsize (sz 0) (sz 15))
-    (sz 9 <: Hax_bounded_integers.t_BoundedUsize (sz 0) (sz 15))
-    (sz 14 <: Hax_bounded_integers.t_BoundedUsize (sz 0) (sz 15))
-    state
+  let state:t_Array u32 (sz 16) = chacha20_quarter_round (sz 0) (sz 4) (sz 8) (sz 12) state in
+  let state:t_Array u32 (sz 16) = chacha20_quarter_round (sz 1) (sz 5) (sz 9) (sz 13) state in
+  let state:t_Array u32 (sz 16) = chacha20_quarter_round (sz 2) (sz 6) (sz 10) (sz 14) state in
+  let state:t_Array u32 (sz 16) = chacha20_quarter_round (sz 3) (sz 7) (sz 11) (sz 15) state in
+  let state:t_Array u32 (sz 16) = chacha20_quarter_round (sz 0) (sz 5) (sz 10) (sz 15) state in
+  let state:t_Array u32 (sz 16) = chacha20_quarter_round (sz 1) (sz 6) (sz 11) (sz 12) state in
+  let state:t_Array u32 (sz 16) = chacha20_quarter_round (sz 2) (sz 7) (sz 8) (sz 13) state in
+  chacha20_quarter_round (sz 3) (sz 4) (sz 9) (sz 14) state
 
 let chacha20_rounds (state: t_Array u32 (sz 16)) : t_Array u32 (sz 16) =
   let st:t_Array u32 (sz 16) = state in
   let st:t_Array u32 (sz 16) =
     Core.Iter.Traits.Iterator.f_fold (Core.Iter.Traits.Collect.f_into_iter #(Core.Ops.Range.t_Range
             i32)
+          #FStar.Tactics.Typeclasses.solve
           ({ Core.Ops.Range.f_start = 0l; Core.Ops.Range.f_end = 10l } <: Core.Ops.Range.t_Range i32
           )
         <:
@@ -129,23 +76,67 @@ let chacha20_core (ctr: u32) (st0: t_Array u32 (sz 16)) : t_Array u32 (sz 16) =
       (Core.Num.impl__u32__wrapping_add (state.[ sz 12 ] <: u32) ctr <: u32)
   in
   let k:t_Array u32 (sz 16) = chacha20_rounds state in
-  Chacha20.Hacspec_helper.add_state state k
+  Core.Array.from_fn #u32
+    (sz 16)
+    (fun i ->
+        let i:usize = i in
+        (state.[ i ] <: u32) +! (k.[ i ] <: u32) <: u32)
+
+let chacha20_key_block (state: t_Array u32 (sz 16)) : t_Array u8 (sz 64) =
+  let state:t_Array u32 (sz 16) = chacha20_core 0ul state in
+  Core.Result.impl__unwrap #(t_Array u8 (sz 64))
+    #Prims.unit
+    (Hax_secret_integers.Traits.f_try_to_le_bytes #(t_Array u32 (sz 16))
+        #u8
+        #(sz 64)
+        #FStar.Tactics.Typeclasses.solve
+        state
+      <:
+      Core.Result.t_Result (t_Array u8 (sz 64)) Prims.unit)
 
 let chacha20_encrypt_block (st0: t_Array u32 (sz 16)) (ctr: u32) (plain: t_Array u8 (sz 64))
     : t_Array u8 (sz 64) =
   let st:t_Array u32 (sz 16) = chacha20_core ctr st0 in
   let (pl: t_Array u32 (sz 16)):t_Array u32 (sz 16) =
-    Chacha20.Hacspec_helper.to_le_u32s_16_ (Rust_primitives.unsize plain <: t_Slice u8)
+    Core.Result.impl__unwrap #(t_Array u32 (sz 16))
+      #Prims.unit
+      (Hax_secret_integers.Traits.f_try_from_le_bytes #(t_Array u32 (sz 16))
+          #u8
+          #FStar.Tactics.Typeclasses.solve
+          (Rust_primitives.unsize plain <: t_Slice u8)
+        <:
+        Core.Result.t_Result (t_Array u32 (sz 16)) Prims.unit)
   in
-  let encrypted:t_Array u32 (sz 16) = Chacha20.Hacspec_helper.xor_state st pl in
-  Chacha20.Hacspec_helper.u32s_to_le_bytes encrypted
+  let (encrypted: t_Array u32 (sz 16)):t_Array u32 (sz 16) =
+    Core.Array.from_fn #u32
+      (sz 16)
+      (fun i ->
+          let i:usize = i in
+          (st.[ i ] <: u32) ^. (pl.[ i ] <: u32) <: u32)
+  in
+  Core.Result.impl__unwrap #(t_Array u8 (sz 64))
+    #Prims.unit
+    (Hax_secret_integers.Traits.f_try_to_le_bytes #(t_Array u32 (sz 16))
+        #u8
+        #(sz 64)
+        #FStar.Tactics.Typeclasses.solve
+        encrypted
+      <:
+      Core.Result.t_Result (t_Array u8 (sz 64)) Prims.unit)
 
 let chacha20_encrypt_last (st0: t_Array u32 (sz 16)) (ctr: u32) (plain: t_Slice u8)
     : Prims.Pure (Alloc.Vec.t_Vec u8 Alloc.Alloc.t_Global)
       (requires (Core.Slice.impl__len #u8 plain <: usize) <=. sz 64)
       (fun _ -> Prims.l_True) =
-  let (b: t_Array u8 (sz 64)):t_Array u8 (sz 64) = Rust_primitives.Hax.repeat 0uy (sz 64) in
-  let b:t_Array u8 (sz 64) = Chacha20.Hacspec_helper.update_array b plain in
+  let (b: t_Array u8 (sz 64)):t_Array u8 (sz 64) =
+    Rust_primitives.Hax.repeat (Hax_secret_integers.Traits.f_classify #u8
+          #FStar.Tactics.Typeclasses.solve
+          0uy
+        <:
+        u8)
+      (sz 64)
+  in
+  let b:t_Array u8 (sz 64) = Core.Slice.impl__copy_from_slice #u8 b plain in
   let b:t_Array u8 (sz 64) = chacha20_encrypt_block st0 ctr b in
   Alloc.Slice.impl__to_vec #u8
     (b.[ {
@@ -160,24 +151,39 @@ let chacha20_encrypt_last (st0: t_Array u32 (sz 16)) (ctr: u32) (plain: t_Slice 
 let chacha20_init (key: t_Array u8 (sz 32)) (iv: t_Array u8 (sz 12)) (ctr: u32)
     : t_Array u32 (sz 16) =
   let (key_u32: t_Array u32 (sz 8)):t_Array u32 (sz 8) =
-    Chacha20.Hacspec_helper.to_le_u32s_8_ (Rust_primitives.unsize key <: t_Slice u8)
+    Core.Result.impl__unwrap #(t_Array u32 (sz 8))
+      #Prims.unit
+      (Hax_secret_integers.Traits.f_try_from_le_bytes #(t_Array u32 (sz 8))
+          #u8
+          #FStar.Tactics.Typeclasses.solve
+          (Rust_primitives.unsize key <: t_Slice u8)
+        <:
+        Core.Result.t_Result (t_Array u32 (sz 8)) Prims.unit)
   in
   let (iv_u32: t_Array u32 (sz 3)):t_Array u32 (sz 3) =
-    Chacha20.Hacspec_helper.to_le_u32s_3_ (Rust_primitives.unsize iv <: t_Slice u8)
+    Core.Result.impl__unwrap #(t_Array u32 (sz 3))
+      #Prims.unit
+      (Hax_secret_integers.Traits.f_try_from_le_bytes #(t_Array u32 (sz 3))
+          #u8
+          #FStar.Tactics.Typeclasses.solve
+          (Rust_primitives.unsize iv <: t_Slice u8)
+        <:
+        Core.Result.t_Result (t_Array u32 (sz 3)) Prims.unit)
   in
   let list =
     [
-      1634760805ul; 857760878ul; 2036477234ul; 1797285236ul; key_u32.[ sz 0 ]; key_u32.[ sz 1 ];
-      key_u32.[ sz 2 ]; key_u32.[ sz 3 ]; key_u32.[ sz 4 ]; key_u32.[ sz 5 ]; key_u32.[ sz 6 ];
-      key_u32.[ sz 7 ]; ctr; iv_u32.[ sz 0 ]; iv_u32.[ sz 1 ]; iv_u32.[ sz 2 ]
+      Hax_secret_integers.Traits.f_classify #u32 #FStar.Tactics.Typeclasses.solve 1634760805ul;
+      Hax_secret_integers.Traits.f_classify #u32 #FStar.Tactics.Typeclasses.solve 857760878ul;
+      Hax_secret_integers.Traits.f_classify #u32 #FStar.Tactics.Typeclasses.solve 2036477234ul;
+      Hax_secret_integers.Traits.f_classify #u32 #FStar.Tactics.Typeclasses.solve 1797285236ul;
+      key_u32.[ sz 0 ]; key_u32.[ sz 1 ]; key_u32.[ sz 2 ]; key_u32.[ sz 3 ]; key_u32.[ sz 4 ];
+      key_u32.[ sz 5 ]; key_u32.[ sz 6 ]; key_u32.[ sz 7 ];
+      Hax_secret_integers.Traits.f_classify #u32 #FStar.Tactics.Typeclasses.solve ctr;
+      iv_u32.[ sz 0 ]; iv_u32.[ sz 1 ]; iv_u32.[ sz 2 ]
     ]
   in
   FStar.Pervasives.assert_norm (Prims.eq2 (List.Tot.length list) 16);
   Rust_primitives.Hax.array_of_list 16 list
-
-let chacha20_key_block (state: t_Array u32 (sz 16)) : t_Array u8 (sz 64) =
-  let state:t_Array u32 (sz 16) = chacha20_core 0ul state in
-  Chacha20.Hacspec_helper.u32s_to_le_bytes state
 
 let chacha20_key_block0 (key: t_Array u8 (sz 32)) (iv: t_Array u8 (sz 12)) : t_Array u8 (sz 64) =
   let state:t_Array u32 (sz 16) = chacha20_init key iv 0ul in
@@ -191,6 +197,7 @@ let chacha20_update (st0: t_Array u32 (sz 16)) (m: t_Slice u8)
   let blocks_out:Alloc.Vec.t_Vec u8 Alloc.Alloc.t_Global =
     Core.Iter.Traits.Iterator.f_fold (Core.Iter.Traits.Collect.f_into_iter #(Core.Ops.Range.t_Range
             usize)
+          #FStar.Tactics.Typeclasses.solve
           ({ Core.Ops.Range.f_start = sz 0; Core.Ops.Range.f_end = num_blocks }
             <:
             Core.Ops.Range.t_Range usize)
@@ -207,6 +214,7 @@ let chacha20_update (st0: t_Array u32 (sz 16)) (m: t_Slice u8)
                   #Core.Array.t_TryFromSliceError
                   (Core.Convert.f_try_into #(t_Slice u8)
                       #(t_Array u8 (sz 64))
+                      #FStar.Tactics.Typeclasses.solve
                       (m.[ {
                             Core.Ops.Range.f_start = sz 64 *! i <: usize;
                             Core.Ops.Range.f_end = (sz 64 *! i <: usize) +! sz 64 <: usize
@@ -259,7 +267,11 @@ let chacha20_update (st0: t_Array u32 (sz 16)) (m: t_Slice u8)
         Alloc.Vec.impl_2__extend_from_slice #u8
           #Alloc.Alloc.t_Global
           blocks_out
-          (Core.Ops.Deref.f_deref #(Alloc.Vec.t_Vec u8 Alloc.Alloc.t_Global) b <: t_Slice u8)
+          (Core.Ops.Deref.f_deref #(Alloc.Vec.t_Vec u8 Alloc.Alloc.t_Global)
+              #FStar.Tactics.Typeclasses.solve
+              b
+            <:
+            t_Slice u8)
       in
       blocks_out
     else blocks_out
